vera/EquivalenceTop.v
@@ -20,7 +20,7 @@ Local Open Scope string.
 Definition sort_vmodule (v : Verilog.vmodule) : string + Verilog.vmodule :=
   trace ("Sort " ++ Verilog.modName v) (
     let* sorted_body :=
-      match sort_module_items (VarSet.of_list (Verilog.module_inputs v)) (Verilog.modBody v) with
+      match sort_module_items (LocationSet.of_varset (VarSet.of_list (Verilog.module_inputs v))) (Verilog.modBody v) with
       | None => inl "Module not sortable"
       | Some sorted => inr sorted
       end in
